src/itree/ITreeLang.v
@@ -51,22 +51,19 @@ Module MemE.
   .
 
   Variant t: Type -> Type :=
-  | read (loc: Loc.t) (ord: Ordering.t): t Const.t 
-  | write (loc: Loc.t) (val: Const.t) (ord: Ordering.t): t unit 
+  | read (loc: Loc.t) (ord: Ordering.t): t Const.t
+  | write (loc: Loc.t) (val: Const.t) (ord: Ordering.t): t unit
   | update (loc: Loc.t) (rmw:rmw) (ordr ordw: Ordering.t): t Const.t
   | fence (ordr ordw: Ordering.t): t unit
   | syscall (args: list Const.t): t Const.t
   | abort: t unit
+  | choose: t Const.t
   .
 End MemE.
 
-Set Implicit Arguments.
 
 
-
-Module State.
-  Definition t := itree MemE.t Const.t.
-
+Module ILang.
   Definition eval_rmw (rmw:MemE.rmw) (val:Const.t): Const.t * option Const.t :=
     match rmw with
     | MemE.fetch_add addendum =>
@@ -80,64 +77,83 @@ Module State.
   Definition is_terminal R (s: itree MemE.t R): Prop :=
     exists r, s = Ret r.
 
-  Inductive step: 
+  Inductive step:
     forall R (e:ProgramEvent.t) (s1: itree MemE.t R) (s2: itree MemE.t R), Prop :=
   | step_tau
-      R (itr: itree MemE.t R):
+      R (itr: itree MemE.t R)
+      itr1 (EQ: itr1 = itr)
+    :
       @step R ProgramEvent.silent
-                  (Tau itr)
-                  itr
+            (Tau itr)
+            itr1
+  | step_choose
+      R (k: Const.t -> itree MemE.t R) val
+      itr1 (EQ: itr1 = k val)
+    :
+      @step R ProgramEvent.silent
+            (Vis (MemE.choose) k)
+            itr1
   | step_read
-      R (k: Const.t -> itree MemE.t R) loc val ord k: 
+      R (k: Const.t -> itree MemE.t R) loc val ord
+      itr1 (EQ: itr1 = k val)
+    :
       @step R (ProgramEvent.read loc val ord)
-                  (Vis (MemE.read loc ord) k)
-                  (k val)
+            (Vis (MemE.read loc ord) k)
+            itr1
   | step_write
-      R (k: unit -> itree MemE.t R) loc val ord k: 
+      R (k: unit -> itree MemE.t R) loc val ord
+      itr1 (EQ: itr1 = k tt)
+    :
       @step R (ProgramEvent.write loc val ord)
-                  (Vis (MemE.write loc val ord) k)
-                  (k tt)
+            (Vis (MemE.write loc val ord) k)
+            itr1
   | step_update_success
       R (k: Const.t -> itree MemE.t R) loc rmw valr valw valret ordr ordw
       (RMW: eval_rmw rmw valr = (valret, Some valw))
-    : 
+      itr1 (EQ: itr1 = k valret)
+    :
       @step R (ProgramEvent.update loc valr valw ordr ordw)
-                  (Vis (MemE.update loc rmw ordr ordw) k)
-                  (k valret)
+            (Vis (MemE.update loc rmw ordr ordw) k)
+            itr1
   | step_update_failure
       R (k: Const.t -> itree MemE.t R) loc rmw valr valret ordr ordw
       (RMW: eval_rmw rmw valr = (valret, None))
-    : 
+      itr1 (EQ: itr1 = k valret)
+    :
       @step R (ProgramEvent.read loc valr ordr)
-                  (Vis (MemE.update loc rmw ordr ordw) k)
-                  (k valret)
+            (Vis (MemE.update loc rmw ordr ordw) k)
+            itr1
   | step_fence
       R (k: unit -> itree MemE.t R) ordr ordw
-    : 
+      itr1 (EQ: itr1 = k tt)
+    :
       @step R (ProgramEvent.fence ordr ordw)
-                  (Vis (MemE.fence ordr ordw) k)
-                  (k tt)
+            (Vis (MemE.fence ordr ordw) k)
+            itr1
   | step_syscall
       R (k: Const.t -> itree MemE.t R) valret args
-    : 
+      itr1 (EQ: itr1 = k valret)
+    :
       @step R (ProgramEvent.syscall (Event.mk valret args))
-                  (Vis (MemE.syscall args) k)
-                  (k valret)
+            (Vis (MemE.syscall args) k)
+            itr1
   | step_abort
       R (k: unit -> itree MemE.t R)
-    : 
+      itr1 (EQ: itr1 = k tt)
+    :
       @step R (ProgramEvent.failure)
-                  (Vis (MemE.abort) k)
-                  (k tt)
+            (Vis (MemE.abort) k)
+            itr1
   .
-End State.
+  #[export] Hint Constructors step: core.
+End ILang.
 
-Definition lang: Language.t ProgramEvent.t :=
+Definition lang (R: Type): Language.t ProgramEvent.t :=
   @Language.mk
     _
-    State.t
-    State.t
+    (itree MemE.t R)
+    (itree MemE.t R)
     id
-    (@State.is_terminal _)
-    (@State.step _)
+    (@ILang.is_terminal _)
+    (@ILang.step _)
 .
